Main.lean
@@ -1,40 +1,21 @@
 import FokkerChallenge
 
 def main : IO Unit := do
-  let mut terms := []
-  terms := terms ++ Cslib.LambdaCalculus.LocallyNameless.Untyped.Term.gen_terms 2 0 0
-
-  terms := terms ++ Cslib.LambdaCalculus.LocallyNameless.Untyped.Term.gen_terms 3 0 0
-  terms := terms ++ Cslib.LambdaCalculus.LocallyNameless.Untyped.Term.gen_terms 2 1 0
-
-  terms := terms ++ Cslib.LambdaCalculus.LocallyNameless.Untyped.Term.gen_terms 4 0 0
-  terms := terms ++ Cslib.LambdaCalculus.LocallyNameless.Untyped.Term.gen_terms 3 1 0
-  terms := terms ++ Cslib.LambdaCalculus.LocallyNameless.Untyped.Term.gen_terms 2 2 0
-
-  terms := terms ++ Cslib.LambdaCalculus.LocallyNameless.Untyped.Term.gen_terms 5 0 0
-  terms := terms ++ Cslib.LambdaCalculus.LocallyNameless.Untyped.Term.gen_terms 4 1 0
-  terms := terms ++ Cslib.LambdaCalculus.LocallyNameless.Untyped.Term.gen_terms 3 2 0
-  terms := terms ++ Cslib.LambdaCalculus.LocallyNameless.Untyped.Term.gen_terms 2 3 0
-
-  terms := terms ++ Cslib.LambdaCalculus.LocallyNameless.Untyped.Term.gen_terms 6 0 0
-  terms := terms ++ Cslib.LambdaCalculus.LocallyNameless.Untyped.Term.gen_terms 5 1 0
-  terms := terms ++ Cslib.LambdaCalculus.LocallyNameless.Untyped.Term.gen_terms 4 2 0
-  terms := terms ++ Cslib.LambdaCalculus.LocallyNameless.Untyped.Term.gen_terms 3 3 0
-  terms := terms ++ Cslib.LambdaCalculus.LocallyNameless.Untyped.Term.gen_terms 2 4 0
+  let terms := Cslib.LambdaCalculus.LocallyNameless.Untyped.Term.terms_fokker_lt_7
 
   -- let len := terms.length
   -- IO.println s!"Solution: {len}"
 
-  terms := terms.filter Cslib.LambdaCalculus.LocallyNameless.Untyped.Term.no_redex
+  let terms := terms.filter Cslib.LambdaCalculus.LocallyNameless.Untyped.Term.no_redex
   -- let len := terms.length
   -- IO.println s!"Solution: {len}"
 
-  terms := terms.filter (fun t => !Cslib.LambdaCalculus.LocallyNameless.Untyped.Term.every_bvar_used t)
+  let terms := terms.filter (fun t => !Cslib.LambdaCalculus.LocallyNameless.Untyped.Term.every_bvar_used t)
   -- let len := terms.length
   -- IO.println s!"Solution: {len}"
 
-  terms := terms.filter (fun t => !Cslib.LambdaCalculus.LocallyNameless.Untyped.Term.no_duplicate t)
-  terms := terms.filter (fun t => !Cslib.LambdaCalculus.LocallyNameless.Untyped.Term.all0_no_fvar_inside_abs t)
+  let terms := terms.filter (fun t => !Cslib.LambdaCalculus.LocallyNameless.Untyped.Term.no_duplicate t)
+  let terms := terms.filter (fun t => !Cslib.LambdaCalculus.LocallyNameless.Untyped.Term.all0_no_fvar_inside_abs t)
   let len := terms.length
   IO.println s!"{len} undecided"
   IO.println s!"{terms}"
